compiler/backend/backend_passesScript.sml
@@ -129,7 +129,9 @@ Definition to_bvi_all_def:
     let (loc,code,n1) = bvl_to_bvi$compile_prog start 0 prog in
     let (n2,code2) = bvi_tailrec$compile_prog c0.do_tailrec (bvl_num_stubs + 2) code in
     let (n3,code3) = bvi_tmc$compile_prog c0.do_tmc (bvl_num_stubs + 3) code2 in
-    let (bvi_inlines,code') = bvi_inline$compile_prog code3 in
+    let ((n4,cm),code4) =
+      bvi_cpr$compile_prog c0.do_cpr (bvl_num_stubs + 4, LN) code3 in
+    let (bvi_inlines,code') = bvi_inline$compile_prog code4 in
     let (s,p,l,bl,n1,n2,n3,names) =
       (loc,code',inlines,bvi_inlines,n1,n2,n3,get_names (MAP FST code') names) in
     let names = sptree$union (sptree$fromAList $ (data_to_word$stub_names () ++
@@ -138,11 +140,13 @@ Definition to_bvi_all_def:
     let ps = ps ++ [(«after bvl_to_bvi»,Bvi code names)] in
     let ps = ps ++ [(«after bvi_tailrec»,Bvi code2 names)] in
     let ps = ps ++ [(«after bvi_tmc»,Bvi code3 names)] in
+    let ps = ps ++ [(«after bvi_cpr»,Bvi code4 names)] in
     let ps = ps ++ [(«after bvi_inline»,Bvi code' names)] in
     let c = c with clos_conf updated_by (λc. c with start := s) in
     let c = c with bvl_conf updated_by
       (λc. c with <| inlines := l; bvi_inlines := bl;
-                    next_name1 := n1; next_name2 := n2; next_name3 := n3 |>) in
+                    next_name1 := n1; next_name2 := n2; next_name3 := n3;
+                    next_name4 := n4; cpr_map := cm |>) in
      ((ps: (mlstring # 'a any_prog) list),c,p,names)
 End
 
@@ -477,7 +481,7 @@ Proof
 QED
 
 Theorem number_of_passes:
-  LENGTH (FST (to_target_all asm_conf c p)) = 41
+  LENGTH (FST (to_target_all asm_conf c p)) = 42
 Proof
   fs [to_target_all_def] \\ rpt (pairarg_tac \\ gvs [])
   \\ fs [to_lab_all_def] \\ rpt (pairarg_tac \\ gvs [])
